deps/poulet4/lib/P4automata/WP.v
@@ -1,74 +1,75 @@
 Require Import Coq.Lists.List.
+Require Import Coq.Classes.EquivDec.
 Require Poulet4.P4automata.Syntax.
 Module P4A := Poulet4.P4automata.Syntax.
 Require Import Poulet4.P4automata.PreBisimulationSyntax.
 
 Section WeakestPre.
-  Variable (a: P4A.t).
-  Variable (has_extract: forall s H, 0 < P4A.size a (exist _ s H)).
+  (* State identifiers. *)
+  Variable (S: Type).
+  Context `{S_eq_dec: EquivDec.EqDec S eq}.
 
-  Definition state_ref_eqb (x y: P4A.state_ref) : bool :=
-    match x, y with
-    | inr b, inr b' => Bool.eqb b b'
-    | inl P4A.SNStart, inl P4A.SNStart => true
-    | inl (P4A.SNName s), inl (P4A.SNName s') => String.eqb s s'
-    | _, _ => false
-    end.
+  (* Header identifiers. *)
+  Variable (H: Type).
+  Context `{H_eq_dec: EquivDec.EqDec H eq}.
 
-  Definition proj_state_type_ref (x: P4A.state_type a + bool) : P4A.state_ref :=
+  Variable (a: P4A.t S H).
+  Variable (has_extract: forall s H, 0 < P4A.size (a:=a) (exist _ s H)).
+
+  Definition proj_state_type_ref (x: P4A.state_type a + bool) : P4A.state_ref S :=
     match x with
     | inr b => inr b
     | inl s => inl (proj1_sig s)
     end.
 
-  Definition expr_to_bit_expr (s: side) (e: P4A.expr) : bit_expr :=
+  Definition expr_to_bit_expr (s: side) (e: P4A.expr H) : bit_expr H :=
     match e with
     | P4A.EHdr h => BEHdr s h
-    | P4A.ELit bs => BELit bs
+    | P4A.ELit _ bs => BELit _ bs
     end.
 
-  Definition val_to_bit_expr (value: P4A.v) : bit_expr :=
+  Definition val_to_bit_expr (value: P4A.v) : bit_expr H :=
     match value with
-    | P4A.VBits bs => BELit bs
+    | P4A.VBits bs => BELit _ bs
     end.
 
-  Definition case_cond (cond: bit_expr) (st': P4A.state_ref) (s: P4A.sel_case) :=
-    if state_ref_eqb st' (P4A.sc_st s)
+  Definition case_cond (cond: bit_expr H) (st': P4A.state_ref S) (s: P4A.sel_case S) :=
+    if st' == P4A.sc_st s
     then BREq cond (val_to_bit_expr (P4A.sc_val s))
-    else BRFalse.
+    else BRFalse _.
 
-  Definition cases_cond (cond: bit_expr) (st': P4A.state_ref) (s: list P4A.sel_case) :=
-    List.fold_right BROr BRFalse (List.map (case_cond cond st') s).
+  Definition cases_cond (cond: bit_expr H) (st': P4A.state_ref S) (s: list (P4A.sel_case S)) :=
+    List.fold_right (@BROr H) (BRFalse _) (List.map (case_cond cond st') s).
 
-  Fixpoint case_negated_conds (cond: bit_expr) (s: list P4A.sel_case) :=
+  Fixpoint case_negated_conds (cond: bit_expr H) (s: list (P4A.sel_case S)) :=
     match s with
-    | nil => BRTrue
+    | nil => BRTrue _
     | s :: rest =>
       BRAnd
         (BRNotEq cond (val_to_bit_expr (P4A.sc_val s)))
         (case_negated_conds cond rest)
     end.
 
-  Definition trans_cond (s: side) (t: P4A.transition) (st': P4A.state_ref) :=
+  Definition trans_cond (s: side) (t: P4A.transition S H) (st': P4A.state_ref S) :=
     match t with
-    | P4A.TGoto r =>
-      if state_ref_eqb r st'
-      then BRTrue
-      else BRFalse
+    | P4A.TGoto _ r =>
+      if r == st'
+      then BRTrue _
+      else BRFalse _
     | P4A.TSel cond cases default =>
       let be_cond := expr_to_bit_expr s cond in
       BROr (cases_cond be_cond st' cases)
-           (if state_ref_eqb default st'
+           (if default == st'
             then case_negated_conds be_cond cases
-            else BRFalse)
+            else BRFalse _)
     end.
 
-  Fixpoint bit_expr_subst (s: side) (h: P4A.hdr_ref) (exp: bit_expr) (phi: bit_expr) : bit_expr :=
+  Fixpoint bit_expr_subst (s: side) (h: P4A.hdr_ref H) (exp: bit_expr H) (phi: bit_expr H) : bit_expr H :=
     match phi with
-    | BELit _
-    | BEBuf _ => phi
+    | BELit _ _
+    | BEBuf _ _ => phi
     | BEHdr s' h' =>
-      if andb (side_beq s s') (Syntax.hdr_ref_beq h h')
+      if andb (s ==b s') (h ==b h')
       then exp
       else phi
     | BESlice e hi lo =>
@@ -78,10 +79,10 @@ Section WeakestPre.
                (bit_expr_subst s h exp e2)
     end.
 
-  Fixpoint store_rel_subst (s: side) (h: P4A.hdr_ref) (exp: bit_expr) (phi: store_rel) : store_rel :=
+  Fixpoint store_rel_subst (s: side) (h: P4A.hdr_ref H) (exp: bit_expr H) (phi: store_rel H) : store_rel H :=
     match phi with
-    | BRTrue
-    | BRFalse =>
+    | BRTrue _
+    | BRFalse _ =>
       phi
     | BREq e1 e2 =>
       BREq (bit_expr_subst s h exp e1)
@@ -97,24 +98,24 @@ Section WeakestPre.
            (store_rel_subst s h exp r2)
     end.
 
-  Fixpoint wp_op' (s: side) (o: P4A.op) : nat * store_rel -> nat * store_rel :=
+  Fixpoint wp_op' (s: side) (o: P4A.op H) : nat * store_rel H -> nat * store_rel H :=
     fun '(buf_idx, phi) =>
       match o with
-      | P4A.OpNil => (buf_idx, phi)
+      | P4A.OpNil _ => (buf_idx, phi)
       | P4A.OpSeq o1 o2 =>
         wp_op' s o1 (wp_op' s o2 (buf_idx, phi))
       | P4A.OpExtract width hdr =>
         let new_idx := buf_idx + width - 1 in
-        let slice := BESlice (BEBuf s) new_idx buf_idx in
+        let slice := BESlice (BEBuf _ s) new_idx buf_idx in
         (new_idx, store_rel_subst s hdr slice phi)
       | P4A.OpAsgn lhs rhs =>
         (buf_idx, store_rel_subst s lhs (expr_to_bit_expr s rhs) phi)
       end.
 
-  Definition wp_op (s: side) (o: P4A.op) (phi: store_rel) : store_rel :=
+  Definition wp_op (s: side) (o: P4A.op H) (phi: store_rel H) : store_rel H :=
     snd (wp_op' s o (0, phi)).
 
-  Definition preds (s: P4A.state_ref) :=
+  Definition preds (s: P4A.state_ref S) :=
     P4A.list_states a.
 
   Definition pick_template (s: side) (c: conf_state a) : state_template a :=
@@ -123,15 +124,15 @@ Section WeakestPre.
     | Right => c.(cs_st2)
     end.
   
-  Definition wp_edge (c: conf_rel a) (s: side) (st: P4A.state) : store_rel :=
+  Definition wp_edge (c: conf_rel a) (s: side) (st: P4A.state S H) : store_rel H :=
     let st' := pick_template s c.(cr_st) in
     let tcond := trans_cond Left (P4A.st_trans st) (proj_state_type_ref st'.(st_state)) in
     let wp_trans := BRAnd c.(cr_rel) tcond in
     wp_op s (P4A.st_op st) wp_trans.
 
-  Definition wp_edges (c: conf_rel a) (s_left: P4A.state_type a) (s_right: P4A.state_type a) : store_rel :=
-    let state_left := P4A.find_state a s_left in
-    let state_right := P4A.find_state a s_right in
+  Definition wp_edges (c: conf_rel a) (s_left: P4A.state_type a) (s_right: P4A.state_type a) : store_rel H :=
+    let state_left := P4A.find_state s_left in
+    let state_right := P4A.find_state s_right in
     let c' := {| cr_st := c.(cr_st);
                  cr_rel := wp_edge c Left state_left |} in
     wp_edge c' Right state_right.
